galois/network/network_local_abs.lean
@@ -7,38 +7,9 @@ import .action
 namespace network
 namespace loc
 
-inductive poll_receive_dlabel_abs (ports : list port) (sockets : list socket)
-    : Type
-| receive_message {} : sockets.member → message_t → poll_receive_dlabel_abs
-
-@[reducible]
-def dlabel' {a} := @dlabel a poll_receive_dlabel_abs
-
-section
-parameters (a_ip : ip) (ag : agent)
-
-def next_receive_dlabel {ports : list port} {sockets : list socket}
-  {bound : time}
-  (cont : poll_result ports sockets bound → list (socket × message_t) × ag.state_type)
-  (elapsed_fin : fin bound) (rn : remote_name)
-  : poll_receive_dlabel_abs ports sockets
-  → list (socket × message_t) × ag.state_type
-| (poll_receive_dlabel_abs.receive_message sock mess) := 
-     cont (poll_result.message elapsed_fin sock mess)
-
-def next_poll_dlabel {ports : list port} {sockets : list socket}
-  {bound : time} (cont : poll_result ports sockets bound → list (socket × message_t) × ag.state_type)
-  : @poll_dlabel poll_receive_dlabel_abs ports sockets bound 
-  → list (socket × message_t) × ag.state_type
-| poll_dlabel.timeout := cont poll_result.timeout
-| (poll_dlabel.receive elapsed_fin rn rlabel) := next_receive_dlabel
-     cont elapsed_fin rn rlabel
-
-def next_agent_state_from_dlabel
-  : ∀ (a_next : act ag.state_type) (la : dlabel' a_next)
-  , ag.state_type
-| (act.poll ports sockets bound cont) (dlabel.poll ._ ._ ._ ._ ms plabel)
-    := (next_poll_dlabel cont plabel).snd
+def next_agent_state_from_dlabel {A} {a_next : act A} (la : dlabel a_next)
+  : A
+  := la.cont_result.snd 
 
 inductive sends_message_st (P : socket → message_t → Prop) : agent_label → Prop
 | mk : ∀ sock mess plabel ms, P sock mess
@@ -46,14 +17,14 @@ inductive sends_message_st (P : socket → message_t → Prop) : agent_label →
      → sends_message_st (agent_label.poll plabel ms)
 
 inductive sends_message_std (P : socket → message_t → Prop) {ag : agent}
-  : ∀ (a_next : act ag.state_type), dlabel' a_next → Prop
-| mk : ∀ ports sockets bound cont ms plabel sock mess, P sock mess
-     → (sock, mess) ∈ ms
-     → sends_message_std (act.poll ports sockets bound cont)
-       (@dlabel.poll ag _ ports sockets bound cont ms plabel)
+  (a_next : act ag.state_type) (la : dlabel a_next) : Prop
+| mk : ∀ sock mess, (sock, mess) ∈ la.messages → sends_message_std
 
-def inLabeld {ag : agent} (P : ∀ (a_next : act ag.state_type), dlabel' a_next → Prop)
-  (x : sigma (λ s : ag.state_type, dlabel' (ag.loop s))) : Prop
+section
+parameters {ag : agent}
+
+def inLabeld (P : ∀ (a_next : act ag.state_type), dlabel a_next → Prop)
+  (x : sigma (λ s : ag.state_type, dlabel (ag.loop s))) : Prop
 := begin
 induction x, apply P; assumption
 end
@@ -70,9 +41,9 @@ induction H,
 { admit }
 end
 
-def LTSd s l s' := next_agent_state_from_dlabel (ag.loop s) l = s'
-
 end
+
+def LTSd (ag : agent) s l s' := @next_agent_state_from_dlabel ag.state_type (ag.loop s) l = s'
 
 end loc
 end network
